Added more wp laws and deeper support for Z-like operations

ITree_CSP.thy
@@ -12,6 +12,9 @@ definition skip :: "('e, unit) itree" where
 definition inp_in :: "('a \<Longrightarrow>\<^sub>\<triangle> 'e) \<Rightarrow> 'a set \<Rightarrow> ('e, 'a) itree" where
 "inp_in c A = (\<bbar> e \<in> (dom match\<^bsub>c\<^esub> \<inter> build\<^bsub>c\<^esub> ` A) \<rightarrow> \<cmark> (the (match\<^bsub>c\<^esub> e)))"
 
+definition inp_where :: "('a \<Longrightarrow>\<^sub>\<triangle> 'e) \<Rightarrow> ('a \<Rightarrow> bool) \<Rightarrow> ('e, 'a) itree" where
+"inp_where c P = Vis (\<lambda> e \<in> dom match\<^bsub>c\<^esub> | P (the (match\<^bsub>c\<^esub> e)) \<bullet> \<cmark> (the (match\<^bsub>c\<^esub> e)))"
+
 lemma retvals_inp_in: "wb_prism c \<Longrightarrow> \<^bold>R(inp_in c A) = A"
   by (auto simp add: inp_in_def)
      (metis imageI insertCI option.sel rangeI retvals_Ret wb_prism.range_build wb_prism_def)
@@ -27,6 +30,11 @@ definition inp_list :: "('a \<Longrightarrow>\<^sub>\<triangle> 'e) \<Rightarrow
 
 definition inp' :: "('a \<Longrightarrow>\<^sub>\<triangle> 'e)\<Rightarrow> ('e, 'a) itree" where
 "inp' c = Vis (pfun_of_map (\<lambda> e. case match\<^bsub>c\<^esub> e of Some v \<Rightarrow> Some (Ret v) | None \<Rightarrow> None))"
+
+lemma inp_where_code [code]:
+  "inp_where c P = Vis (pfun_of_map (\<lambda> e. case match\<^bsub>c\<^esub> e of Some v \<Rightarrow> if (P v) then Some (Ret v) else None | None \<Rightarrow> None))"
+  by (auto simp add: inp_where_def fun_eq_iff pfun_eq_iff domI pdom.abs_eq option.case_eq_if)
+     (metis option.collapse option.distinct(1))+
 
 lemma build_in_dom_match [simp]: "wb_prism c \<Longrightarrow> build\<^bsub>c\<^esub> x \<in> dom match\<^bsub>c\<^esub>"
   by (simp add: dom_def)
